feat: geometric constructions

ProofWidgets/Demos/Euclidean.lean
@@ -1,7 +1,7 @@
 /-
  Copyright (c) 2023 Vladimir Sedlacek. All rights reserved.
  Released under Apache 2.0 license as described in the file LICENSE.
- Authors: Vladimir Sedlacek
+ Authors: Vladimir Sedlacek, Wojciech Nawrocki
  -/
 
 import Lean.Data.HashMap
@@ -10,21 +10,29 @@ import ProofWidgets.Component.PenroseDiagram
 import ProofWidgets.Component.HtmlDisplay
 import ProofWidgets.Component.Panel.Basic
 import ProofWidgets.Component.OfRpcMethod
+import ProofWidgets.Component.MakeEditLink
+
+/-! A widget to display Euclidean geometry diagrams,
+and another one to make geometric constructions in the UI. -/
 
 open Lean Meta Server
 open ProofWidgets
 
-/-! # Minimal definitions of synthetic geometric primitives, inspired by https://github.com/ah1112/synthetic_euclid_4 -/
+/-! # Minimal definitions of synthetic geometric primitives
+
+Inspired by https://github.com/ah1112/synthetic_euclid_4. -/
 
 class IncidenceGeometry where
   Point : Type u₁
   Line : Type u₂
-
   between : Point → Point → Point → Prop -- implies colinearity
   onLine : Point → Line → Prop
   ne_23_of_between : ∀ {a b c : Point}, between a b c → b ≠ c
-  line_unique_of_pts : ∀ {a b : Point}, ∀ {L M : Line}, a ≠ b → onLine a L → onLine b L → onLine a M → onLine b M → L = M
-  onLine_2_of_between : ∀ {a b c : Point}, ∀ {L : Line}, between a b c → onLine a L → onLine c L → onLine b L
+  line_unique_of_pts : ∀ {a b : Point}, ∀ {L M : Line},
+    a ≠ b → onLine a L → onLine b L → onLine a M → onLine b M → L = M
+  onLine_2_of_between : ∀ {a b c : Point}, ∀ {L : Line},
+    between a b c → onLine a L → onLine c L → onLine b L
+  line_of_pts : ∀ a b, ∃ L, onLine a L ∧ onLine b L
 
 variable [i : IncidenceGeometry]
 open IncidenceGeometry
@@ -41,83 +49,123 @@ def isBetweenPred? (e : Expr) : Option (Expr × Expr × Expr) := do
   let some (_, a, b, c) := e.app4? ``between | none
   return (a, b, c)
 
-/-- Expressions to display as labels in a diagram. -/
-abbrev ExprEmbeds := Array (String × Expr)
+def isPoint? (e : Expr) : Bool :=
+  e.isAppOf ``Point
+
+def isLine? (e : Expr) : Bool :=
+  e.isAppOf ``Line
+
+/-! # Utilities for constructing diagrams -/
+
+structure DiagramState where
+  /-- The Penrose substance program.
+  Note that `embeds` are added lazily at the end. -/
+  sub : String := ""
+  /-- Components to display as labels in the diagram,
+  mapped as name ↦ (type, html). -/
+  embeds : HashMap String (String × Html) := .empty
+
+abbrev DiagramBuilderM := StateT DiagramState MetaM
 
 open scoped Jsx in
-def mkEuclideanDiag (sub : String) (embeds : ExprEmbeds) : MetaM Html := do
-  let embeds ← embeds.mapM fun (s, h) =>
-      return (s, <InteractiveCode fmt={← Widget.ppExprTagged h} />)
-  return (
-    <PenroseDiagram
-      embeds={embeds}
-      dsl={include_str ".."/".."/"widget"/"penrose"/"euclidean.dsl"}
-      sty={include_str ".."/".."/"widget"/"penrose"/"euclidean.sty"}
-      sub={sub} />)
-
-def isEuclideanGoal? (hyps : Array LocalDecl) : MetaM (Option Html) := do
+def buildDiagram : DiagramBuilderM (Option Html) := do
+  let st ← get
+  if st.sub == "" && st.embeds.isEmpty then
+    return none
   let mut sub := "AutoLabel All\n"
-  let mut sets : HashMap String Expr := .empty
-  for assm in hyps do
-    let tp ← instantiateMVars assm.type
+  let mut embedHtmls := #[]
+  for (n, (tp, h)) in st.embeds.toArray do
+    sub := sub ++ s!"{tp} {n}\n"
+    embedHtmls := embedHtmls.push (n, h)
+  sub := sub ++ st.sub
+  return <PenroseDiagram
+    embeds={embedHtmls}
+    dsl={include_str ".."/".."/"widget"/"penrose"/"euclidean.dsl"}
+    sty={include_str ".."/".."/"widget"/"penrose"/"euclidean.sty"}
+    sub={sub} />
+
+/-- Add a substance `nm` of Penrose type `tp`,
+labelled by `h` to the substance program. -/
+def addEmbed (nm : String) (tp : String) (h : Html) : DiagramBuilderM Unit := do
+  modify fun st => { st with embeds := st.embeds.insert nm (tp, h )}
+
+open scoped Jsx in
+/-- Add a substance of Penrose type `tp`,
+corresponding to (and labelled by) the expression `e`,
+to the substance program.
+Return its Penrose name. -/
+def addExpr (tp : String) (e : Expr) : DiagramBuilderM String := do
+  let nm ← toString <$> Lean.Meta.ppExpr e
+  let h := <InteractiveCode fmt={← Widget.ppExprTagged e} />
+  addEmbed nm tp h
+  return nm
+
+def addExpr' (tp : String) (e : Expr) : DiagramBuilderM Unit := do
+  let _ ← addExpr tp e
+
+/-- Add instruction `i` to the substance program. -/
+def addInstruction (i : String) : DiagramBuilderM Unit := do
+  modify fun st => { st with sub := st.sub ++ s!"{i}\n" }
+
+def addHypotheses (hyps : Array LocalDecl) : DiagramBuilderM Unit := do
+  for h in hyps do
+    let tp ← instantiateMVars h.type
+    if isPoint? tp then
+      addExpr' "Point" h.toExpr
+    if isLine? tp then
+      addExpr' "Line" h.toExpr
     if let some (a, L) := isOnLinePred? tp then
-      let sa ← toString <$> Lean.Meta.ppExpr a
-      let sL ← toString <$> Lean.Meta.ppExpr L
-      let (sets', ca) := sets.insert' sa a
-      let (sets', cL) := sets'.insert' sL L
-      sets := sets'
-      if !ca then
-        sub := sub ++ s!"Point {sa}\n"
-      if !cL then
-        sub := sub ++ s!"Line {sL}\n"
-      sub := sub ++ s!"On({sa}, {sL})\n"
+      let sa ← addExpr "Point" a
+      let sL ← addExpr "Line" L
+      addInstruction s!"On({sa}, {sL})"
     if let some (a, b, c) := isBetweenPred? tp then
-      let sa ← toString <$> Lean.Meta.ppExpr a
-      let sb ← toString <$> Lean.Meta.ppExpr b
-      let sc ← toString <$> Lean.Meta.ppExpr c
-      let (sets', ca) := sets.insert' sa a
-      let (sets', cb) := sets'.insert' sb b
-      let (sets', cc) := sets'.insert' sc c
-      sets := sets'
-      if !ca then
-        sub := sub ++ s!"Point {sa}\n"
-      if !cb then
-        sub := sub ++ s!"Point {sb}\n"
-      if !cc then
-        sub := sub ++ s!"Point {sc}\n"
-      sub := sub ++ s!"Between({sa}, {sb}, {sc})\n"
-  if sets.isEmpty then return none
-  some <$> mkEuclideanDiag sub sets.toArray
+      let sa ← addExpr "Point" a
+      let sb ← addExpr "Point" b
+      let sc ← addExpr "Point" c
+      addInstruction s!"Between({sa}, {sb}, {sc})"
+
+def DiagramBuilderM.run (x : DiagramBuilderM α) : MetaM α :=
+  x.run' {}
 
 /-! # Implementation of the widget -/
-
-def findGoalForLocation (goals : Array Widget.InteractiveGoal) (loc : SubExpr.GoalsLocation) :
-    Option Widget.InteractiveGoal :=
-  goals.find? (·.mvarId == loc.mvarId)
 
 open scoped Jsx in
 @[server_rpc_method]
 def EuclideanDisplay.rpc (props : PanelWidgetProps) : RequestM (RequestTask Html) :=
   RequestM.asTask do
     let inner : Html ← (do
-      if props.selectedLocations.isEmpty then
-        return <span>Use shift-click to select hypotheses to include in the diagram.</span>
-      let some selectedLoc := props.selectedLocations[0]? | unreachable!
+      -- Are there any goals unsolved? If so, pick the first one.
+      if props.goals.isEmpty then
+        return <span>No goals.</span>
+      let some g := props.goals[0]? | unreachable!
 
-      let some g := findGoalForLocation props.goals selectedLoc
-        | throw $ .invalidParams
-            s!"could not find goal for location {toJson selectedLoc}"
+      -- Execute the next part using the metavariable context and local context of the goal.
       g.ctx.val.runMetaM {} do
         let md ← g.mvarId.getDecl
         let lctx := md.lctx |>.sanitizeNames.run' {options := (← getOptions)}
         Meta.withLCtx lctx md.localInstances do
-          let locs : Array LocalDecl ← props.selectedLocations.filterMapM fun
+          -- Which hypotheses have been selected in the UI,
+          -- meaning they should *not* be shown in the display.
+          let mut hiddenLocs : HashSet FVarId := mkHashSet props.selectedLocations.size
+          for l in props.selectedLocations do
+            match l with
             | ⟨mv, .hyp fv⟩ | ⟨mv, .hypType fv _⟩ =>
-              return if mv == g.mvarId then some (← fv.getDecl) else none
-            | _ => return none
-          match ← isEuclideanGoal? locs with
-          | some html => return html
-          | none => return <span>No Euclidean goal.</span>)
+              if mv == g.mvarId then
+                hiddenLocs := hiddenLocs.insert fv
+            | _ => continue
+          -- Filter local declarations by whether they are not in `hiddenLocs`.
+          let locs := (← getLCtx).decls.toArray.filterMap (fun d? =>
+            if let some d := d? then
+              if !hiddenLocs.contains d.fvarId then some d else none
+            else
+              none)
+          -- Produce the diagram.
+          DiagramBuilderM.run do
+            addHypotheses locs
+            match ← buildDiagram with
+            | some html => return html
+            | none => return <span>No Euclidean goal.</span>)
+
     return <details «open»={true}>
         <summary className="mv2 pointer">Euclidean diagram</summary>
         <div className="ml1">{inner}</div>
@@ -136,3 +184,91 @@ example {a b c : Point} {L M : Line} (Babc : between a b c) (aL : onLine a L) (b
     have bc := ne_23_of_between Babc
     have bL := onLine_2_of_between Babc aL cL
     exact line_unique_of_pts bc bL cL bM cM
+
+/-! # Euclidean constructions -/
+
+open scoped Jsx in
+/-- Add every possible line between any two points in `hyps`
+to the diagram.
+Lines are labelled with links to insert them into the proof script. -/
+def constructLines (hyps : Array LocalDecl) (meta : Server.DocumentMeta) (cursorPos : Lsp.Position)
+    : DiagramBuilderM Unit := do
+  -- Identify all the points.
+  let mut points : Array LocalDecl := {}
+  for h in hyps do
+    let tp ← instantiateMVars h.type
+    if isPoint? tp then
+      points := points.push h
+
+  -- Construct every possible line.
+  for hi : i in [0:points.size] do
+    for hj : j in [i+1:points.size] do
+      let p := points[i]'hi.upper
+      let q := points[j]'hj.upper
+      let sp ← addExpr "Point" p.toExpr
+      let sq ← addExpr "Point" q.toExpr
+      let nm := s!"{sp}{sq}"
+      let ctr := s!"let ⟨{nm}, _, _⟩ := line_of_pts {sp} {sq}"
+      -- Add the line, labelled with a link that makes the text edit.
+      addEmbed nm "Line" (
+        <span>
+          <b>{.text nm}</b> ({
+            .ofComponent MakeEditLink
+              (MakeEditLinkProps.ofReplaceRange meta ⟨cursorPos, cursorPos⟩ ctr)
+              #[.text "insert"]
+          })
+        </span>)
+      addInstruction s!"On({sp}, {nm})"
+      addInstruction s!"On({sq}, {nm})"
+      addInstruction s!"Emphasize({nm})"
+
+open scoped Jsx in
+@[server_rpc_method]
+def EuclideanConstructions.rpc (props : PanelWidgetProps) : RequestM (RequestTask Html) :=
+  RequestM.asTask do
+    let doc ← RequestM.readDoc
+    let inner : Html ← (do
+      -- Are there any goals unsolved? If so, pick the first one.
+      if props.goals.isEmpty then
+        return <span>No goals.</span>
+      let some g := props.goals[0]? | unreachable!
+
+      -- Execute the next part using the metavariable context and local context of the goal.
+      g.ctx.val.runMetaM {} do
+        let md ← g.mvarId.getDecl
+        let lctx := md.lctx |>.sanitizeNames.run' {options := (← getOptions)}
+        Meta.withLCtx lctx md.localInstances do
+
+          -- Grab all hypotheses from the local context.
+          let allHyps := (← getLCtx).decls.toArray.filterMap id
+
+          -- Find which hypotheses are selected.
+          let selectedHyps ← props.selectedLocations.filterMapM fun
+            | ⟨mv, .hyp fv⟩ | ⟨mv, .hypType fv _⟩ =>
+              return if mv == g.mvarId then some (← fv.getDecl) else none
+            | _ =>
+              return none
+
+          -- Produce the diagram.
+          DiagramBuilderM.run do
+            addHypotheses allHyps
+            constructLines selectedHyps doc.meta props.pos
+            match ← buildDiagram with
+            | some html => return html
+            | none => return <span>No Euclidean goal.</span>)
+
+    -- Return a collapsible `<details>` block around our widget.
+    return <details «open»={true}>
+        <summary className="mv2 pointer">Euclidean constructions</summary>
+        <div className="ml1">{inner}</div>
+      </details>
+
+@[widget_module]
+def EuclideanConstructions : Component PanelWidgetProps :=
+  mk_rpc_widget% EuclideanConstructions.rpc
+
+example {a b c d : Point} : ∃ L, onLine a L ∧ onLine b L := by
+  with_panel_widgets [EuclideanConstructions]
+    -- Place your cursor below.
+
+    sorry
