widget/penrose/euclidean.dsl
@@ -3,3 +3,5 @@ type Line
 
 predicate Between(Point a, Point b, Point c)
 predicate On(Point a, Line L)
+
+predicate Emphasize(Line L)
